secure_api/box/functor_box/Box.PKAE.fst
@@ -34,7 +34,9 @@ module LE = FStar.Endianness
 let nonce = AE.nonce
 let cipher = AE.cipher
 let subId_t = ODH.dh_share
+let plain_max_length = AE.plain_max_length
 let plain_t = AE.ae_plain
+let length = AE.length
 
 //let message_log_range (im:index_module) = AE.message_log_range im
 //let message_log_inv (im:index_module) (pm:plain_module) (f:MM.map' (message_log_key im) (message_log_range im pm)) = AE.message_log_inv im pm f
@@ -42,7 +44,7 @@ let plain_t = AE.ae_plain
 let pkey = ODH.pkey
 let skey = ODH.skey
 
-#set-options "--z3rlimit 1900 --max_ifuel 2 --max_fuel 1"
+#set-options "--z3rlimit 900 --max_ifuel 2 --max_fuel 1"
 private noeq type aux_t' (im:index_module{ID.get_subId im == subId_t}) (pm:plain_module) (rgn:log_region im) =
   | AUX:
     am:AE.ae_module im ->
@@ -52,21 +54,6 @@ private noeq type aux_t' (im:index_module{ID.get_subId im == subId_t}) (pm:plain
 
 let aux_t im pm = aux_t' im pm
 
-
-
-type efun2 (a:Type) (b:Type) (c:Type) = a -> b -> Tot c
-
-type feq2 (#a:Type) (#b:Type) (#c:Type) (f:efun2 a b c) (g:efun2 a b c) =
-(forall x. forall y. {:pattern (f x y) \/ (g x y)} f x y == g x y)
-
-assume Extensionality2 : forall (a:Type) (b:Type) (c:Type) (f: efun2 a b c) (g: efun2 a b c).
-{:pattern feq2 #a #b #c f g} feq2 #a #b #c f g <==> f==g
-
-
-val coerce: t1:Type -> t2:Type{t1 == t2} -> x:t1 -> t2
-let coerce t1 t2 x = x
-
-#set-options "--z3rlimit 200 --max_ifuel 1 --max_fuel 0"
 val message_log_lemma: im:index_module -> rgn:log_region im -> Lemma
   (requires True)
   (ensures message_log im rgn === AE.message_log im rgn)
@@ -85,34 +72,18 @@ let message_log_lemma im rgn =
   ()
 
 
+#set-options "--z3rlimit 100 --max_ifuel 1 --max_fuel 0"
 let get_message_log_region pkm = AE.get_message_log_region pkm.aux.am
+
+val coerce: t1:Type -> t2:Type{t1 == t2} -> x:t1 -> t2
+let coerce t1 t2 x = x
 
 let get_message_logGT pkm =
   let (ae_log:AE.message_log pkm.im (get_message_log_region pkm)) = AE.get_message_logGT #pkm.im pkm.aux.am in
   let (ae_rgn:log_region pkm.im) = AE.get_message_log_region pkm.aux.am in
   message_log_lemma pkm.im ae_rgn;
   let log:message_log pkm.im ae_rgn = coerce (AE.message_log pkm.im ae_rgn) (message_log pkm.im ae_rgn) ae_log in
-  //admit()
   log
-
-
-(* "Box.PKAE.message_log
-    (PKAE?.im pkm)
-    (Box.AE.get_message_log_region (AUX?.am (PKAE?.aux pkm)))"
-
-"(ml:Box.AE.message_log
-    (PKAE?.im pkm)
-    (AM?.message_log_region (AUX?.am (PKAE?.aux pkm)))
-    { ml == AM?.message_log (AUX?.am (PKAE?.aux pkm)) })"
-*)
-// "(ml:Box.AE.message_log (PKAE?.im pkm)
-//  (AM?.message_log_region (AUX?.am (PKAE?.aux pkm)))
-//  { ml == AM?.message_log (AUX?.am (PKAE?.aux pkm)) })"
-//  effect "GTot"
-
-//     "Box.PKAE.message_log (PKAE?.im pkm)
-//  (PKAE?.rgn pkm)"
-//  effect "GTot"
 
 val create_aux: (im:index_module{ID.get_subId im == subId_t}) -> (pm:plain_module{Plain.get_plain pm == plain_t}) -> rgn:log_region im -> St (aux_t im pm rgn)
 let create_aux im pm rgn =
@@ -121,12 +92,17 @@ let create_aux im pm rgn =
   let om = ODH.create im km rgn in
   AUX am km om
 
-let create rgn =
-  let im = ID.create rgn subId_t  in
-  ()
+assume val enc (pm:plain_module): (Plain.get_plain pm) -> n:nonce -> pk:pkey -> sk:skey -> Tot cipher
+assume val dec (pm:plain_module): c:cipher -> n:nonce -> pk:pkey -> sk:skey -> Tot (option (Plain.get_plain pm)) 
 
-let get_message_log pkm =
-  pkm.message_log
+let create rgn =
+  let id_log_rgn : ID.id_log_region = new_region rgn in
+  let im = ID.create id_log_rgn subId_t ODH.smaller ODH.total_order_lemma in
+  let pm = Plain.create plain_t AE.plain_max_length AE.length in
+  let log_rgn : log_region im = new_region rgn in
+  let aux = create_aux im pm log_rgn in
+  PKAE im pm log_rgn (enc pm) (dec pm) aux
+
 
 type key (pkm:pkae_module) = AE.key pkm.im
 
@@ -147,25 +123,17 @@ let compatible_keys sk pk = ODH.compatible_keys sk pk
 
 
 
-#set-options "--z3rlimit 100 --max_ifuel 0 --max_fuel 0"
+#set-options "--z3rlimit 500 --max_ifuel 1 --max_fuel 1"
 let encrypt pkm #i n sk pk m =
   let k = ODH.prf_odh pkm.im pkm.aux.km pkm.aux.om sk pk in
   let c = AE.encrypt pkm.aux.am #i n k m in
   let h = get() in
   assert(FStar.FunctionalExtensionality.feq (message_log_range pkm.im) (AE.message_log_range pkm.im));
-  MM.contains_eq_compat (pkm.message_log) (AE.get_message_logGT pkm.aux.am) (n,i) (c,m) h;
-  MM.contains_stable pkm.message_log (n,i) (c,m);
-  MR.witness pkm.message_log (MM.contains pkm.message_log (n,i) (c,m));
+  MM.contains_eq_compat (get_message_logGT pkm) (AE.get_message_logGT pkm.aux.am) (n,i) (c,m) h;
+  MM.contains_stable (get_message_logGT pkm) (n,i) (c,m);
+  MR.witness (get_message_logGT pkm) (MM.contains (get_message_logGT pkm) (n,i) (c,m));
   c
 
-//val decrypt: pkm:pkae_module -> #i:id pkm -> n:nonce -> sk:skey -> pk:pkey{ODH.compatible_keys sk pk /\ i = ID.compose_ids pkm.im (ODH.pk_get_share pk) (ODH.sk_get_share sk)} -> c:cipher -> ST (option (message pkm i))
-//  (requires (fun h0 ->
-//    registered pkm i
-//    /\ Key.invariant pkm.im pkm.km h0
-//  ))
-//  (ensures  (fun h0 c h1 ->
-//    Key.invariant pkm.im pkm.km h1
-//  ))
 let decrypt pkm #i n sk pk c =
   let k = ODH.prf_odh pkm.im pkm.km pkm.om sk pk in
   let m = AE.decrypt pkm.am #i n k c in
