secure_api/box/functor_box/Box.PKAE.fsti
@@ -31,7 +31,9 @@ type log_region (im:index_module) =
   r:MR.rid{disjoint r (ID.get_rgn im)}
 
 val subId_t: Type0
+val plain_max_length: nat
 val plain_t: Type0
+val length: p:plain_t -> n:nat{n<plain_max_length}
 
 type message_log_key (im:index_module) = (nonce*(i:id im))
 type message_log_value (im:index_module) (i:id im) = (cipher*Plain.protected_plain_t im plain_t i)
@@ -48,7 +50,7 @@ val aux_t: (im:index_module{ID.get_subId im == subId_t}) -> (pm:plain_module{Pla
 abstract noeq type pkae_module =
   | PKAE:
     im:ID.index_module{ID.get_subId im == subId_t} ->
-    pm:Plain.plain_module{Plain.get_plain pm == plain_t} ->
+    pm:Plain.plain_module{Plain.get_plain pm == plain_t /\ Plain.plain_max_length #pm= plain_max_length} ->
     rgn:log_region im ->
     enc: ((Plain.get_plain pm) -> n:nonce -> pk:pkey -> sk:skey -> Tot cipher) ->
     dec: (c:cipher -> n:nonce -> pk:pkey -> sk:skey -> Tot (option (Plain.get_plain pm))) ->
@@ -56,11 +58,12 @@ abstract noeq type pkae_module =
     pkae_module
 
 val get_message_log_region: pkm:pkae_module -> GTot (log_region pkm.im)
-val get_message_logGT: pkm:pkae_module -> GTot (message_log pkm.im (get_message_log_region pkm))
+val get_message_logGT: pkm:pkae_module -> Tot (message_log pkm.im (get_message_log_region pkm)) //TODO: MK: would prefer this to be GTot
 
-val create: #im:index_module -> rgn:log_region im -> pkae_module
+val create: rgn:(r:MR.rid{extends r root /\ is_eternal_region r /\ is_below r root}) -> St (pkae_module)
 
-val zero_bytes: (n:nat) -> b:bytes{Seq.length b = n /\ b=Seq.create n (UInt8.uint_to_t 0)}
+val zero_bytes: (n:nat{n<plain_max_length}) -> plain_t //b:bytes{Seq.length b = n /\ b=Seq.create n (UInt8.uint_to_t 0)}
+//TODO: MK this can be modelled better
 
 val pkey_to_subId: #pkm:pkae_module -> pk:pkey -> ID.get_subId pkm.im
 val pkey_to_subId_inj: #pkm:pkae_module -> pk:pkey -> Lemma
@@ -71,8 +74,8 @@ val pkey_to_subId_inj: #pkm:pkae_module -> pk:pkey -> Lemma
 #set-options "--z3rlimit 2000 --max_ifuel 1 --max_fuel 0"
 val nonce_is_fresh: (pkm:pkae_module) -> (i:id pkm.im) -> (n:nonce) -> (h:mem) ->
   (t:Type0{t <==>
-    (MR.m_contains pkm.message_log h
-    /\ MM.fresh pkm.message_log (n,i) h)})
+    (MR.m_contains #(get_message_log_region pkm) (get_message_logGT pkm) h
+      /\ MM.fresh #(get_message_log_region pkm)(get_message_logGT pkm) (n,i) h)})
 
 val pkey_from_skey: sk:skey -> pk:pkey
 
@@ -109,7 +112,7 @@ val encrypt: pkm:pkae_module ->
     /\ ((dishonest pkm i \/ ~(b2t ae_ind_cpa)) // Concrete behaviour otherwise.
                   ==> (eq2 #cipher c (pkm.enc (Plain.repr #pkm.im #pkm.pm #i m) n pk sk)))
     // The message is added to the log. This also guarantees nonce-uniqueness.
-    /\ MR.m_contains pkm.message_log h1
-    /\ MR.witnessed (MM.contains pkm.message_log (n,i) (c,m))
-    /\ MR.m_sel h1 pkm.message_log == MM.upd (MR.m_sel h0 pkm.message_log) (n,i) (c,m)
+      /\ MR.m_contains #(get_message_log_region pkm)(get_message_logGT pkm) h1
+        /\ MR.witnessed (MM.contains #(get_message_log_region pkm) (get_message_logGT pkm) (n,i) (c,m))
+        /\ MR.m_sel #(get_message_log_region pkm) h1 (get_message_logGT pkm)== MM.upd (MR.m_sel #(get_message_log_region pkm) h0 (get_message_logGT pkm)) (n,i) (c,m)
   ))
